\documentclass{article}

\usepackage[a4paper,top=2cm,bottom=.5cm,left=0.8cm,right=0.8cm]{geometry}
\usepackage[fleqn]{amsmath}
\usepackage{amssymb}
\usepackage{fancyhdr}
\usepackage{mathtools}
\usepackage{booktabs}
\usepackage{multicol}
\usepackage[table,xcdraw]{xcolor}
\usepackage{titlesec}
\usepackage[most]{tcolorbox}

\titlespacing*\subsection{0pt}{0pt}{0pt}
\titlespacing*\subsubsection{0pt}{0pt}{0pt}

\setlength{\headsep}{0.3cm}

\setlength{\abovedisplayskip}{0pt}
\setlength{\belowdisplayskip}{0pt}

\title{MAST20005 Statistics - Summary Notes}
\date{\today}
\author{Lucas Fern (1080613)}
\lhead{MAST20005 Statistics - Summary Notes}
\rhead{Lucas Fern (1080613)}

\pagestyle{fancy}

\begin{document}
\pagenumbering{gobble}
%\begin{table}[h!]
%    \vspace{-0.35cm}
%    \centering
%    \begin{tabular}{@{}llll@{}}
%    \multicolumn{1}{c}{\textbf{Distribution}}       & \multicolumn{1}{c}{\textbf{Probability Density Function}}                                                                          & \multicolumn{1}{c}{\textbf{$\mathbb{E}(X)$}}                & \multicolumn{1}{c}{\textbf{$\mbox{Var}(X)$}}                                                                       \\ \midrule
%    $X \sim \mbox{Bi}(n,p)$                & $p_X(x)={\binom{n}{x}}p^x(1-p)^{n-x}$                                                                                              & $np$                                                        & $np(1-p)$                                                                                                          \\ \midrule
%    $N \sim \mbox{G}(p)$                   & $p_N(n)=(1-p)^{n}p$                                                                                                                & $\frac{1-p}{p}$                                             & $\frac{1-p}{p^2}$                                                                                                  \\ \midrule
%    $Z \sim \mbox{Nb}(r,p)$                & $p_Z(z)={\binom{-r}{z}}p^r(p-1)^z$                                                                                                 &                                                             &                                                                                                                    \\ \midrule
%    $X \sim \mbox{Hg}(n,D,N)$              & $p_X(x)=\frac{{\binom{D}{x}}{\binom{N-D}{n-x}}}{{\binom{N}{n}}}$                                                                   & $\frac{nD}{N}$                                              & $\frac{nD(N-D)}{N^2}\cdot(1-\frac{n-1}{N-1})$                                                                      \\ \midrule
%    $X \sim \mbox{Pn}(\alpha t)$           & $p_X(x)=\frac{e^{-\alpha}(\alpha)^x}{x!}$                                                                                          & $\alpha$                                                    & $\alpha$                                                                                                           \\ \midrule
%    $X \sim \mbox{U}(m,n)$ - Discrete Uniform                 & $p_X(x)=\frac{1}{n-m+1}$                                                                                                           & $\frac{m+n}{2}$                                             & $\frac{1}{12}((n-m+1)^2-1)$                                                                                        \\ \midrule
%    $X \sim \mbox{R}(a,b)$ - Continuous Uniform                & $f_X(x)=\frac{1}{b-a}$                                                                                                             & $\frac{a+b}{2}$                                             & $\frac{1}{12}(b-a)^2$                                                                                              \\ \midrule
%    $T \sim \mbox{exp}(\alpha)$ - Rate Parameter           & $f_T(t)=\alpha e^{-\alpha t}, \mbox{ for } t \geq 0$                                                                               & $\frac{1}{\alpha}$                                          & $\frac{1}{\alpha ^2}$                                                                                              \\[2mm]
%    $T \sim \mbox{exp}(\theta)$ - Scale Parameter           & $f_T(t)=\frac{1}{\theta} e^{-\frac{1}{\theta} t}, \mbox{ for } t \geq 0$                                                                               & $\theta$                                          & $\theta^{2}$                                                                                              \\ \midrule
%    $T \sim \gamma(r,\alpha)$              & $f_T(t)=\frac{\alpha^r t^{r-1} e^{-\alpha t}}{\Gamma(r)}, \mbox{ for } t \geq 0$                                                                  & $\frac{r}{\alpha}$                                          & $\frac{r}{\alpha ^2}$                                                                                              \\ \midrule
%    $X \sim \mbox{Pareto}(\alpha, \gamma)$ & $f_X(x)=\frac{\gamma \alpha^\gamma}{x^{\gamma+1}}, \mbox{ for } \alpha \leq x < \infty$                                            & $\frac{\gamma \alpha}{\gamma - 1}, \mbox{ for } \gamma > 1$ & $\frac{\gamma \alpha^2}{(\gamma-1)^2(\gamma - 2)}, \mbox{ for } \gamma > 2$                                        \\ \midrule
%    $X \sim \mbox{N}(\mu, \sigma^2)$       & $f_X(x)=\frac{1}{\sigma \sqrt{2\pi}}e^{-\frac{1}{2\sigma^2}(x-\mu)^2}, \mbox{ for } x \in \mathbb{R}$                              & $\mu$                                                       & $\sigma^2$                                                                                                         \\ \midrule
%    $X \sim \mbox{Beta}(\alpha, \beta)$       & $f_X(x)=\frac{\Gamma(\alpha + \beta)}{\Gamma(\alpha)\Gamma(\beta)} x^{\alpha - 1} (1 - x)^{\beta - 1}, \mbox{ for } x \in [0, 1]$                              & $\frac{\alpha}{\alpha + \beta}$                                                       & $\frac{\alpha \beta}{(\alpha + \beta)^{2} (\alpha + \beta + 1)}$                                                                                                         \\ \midrule
%    $X \sim \mbox{Weibull}(\beta, \gamma)$ & $f_X(x)=\frac{\gamma x^{\gamma - 1}}{\beta^\gamma}e^{-(\frac{x}{\beta})^\gamma}, \mbox{ for } 0 \leq x < \infty$                   & $\beta \Gamma\left(\frac{\gamma + 1}{\gamma}\right)$        & $\beta^2 \left[\Gamma\left(\frac{\gamma + 2}{\gamma}\right)-\Gamma\left(\frac{\gamma + 1}{\gamma}\right)^2\right]$ \\ \midrule
%    $X \sim \mbox{C}(m, a)$                & $f_X(x)=\frac{1}{\pi} \frac{a}{a^2 + (x-m)^2}, \mbox{ for } -\infty < x < \infty$                                                  & Undefined                                                   & Undefined                                                                                                          \\ \midrule
%    $Y \sim \mbox{LN}(\mu, \sigma^2)$      & $f_Y(y)=\frac{1}{\sqrt{2\pi}\sigma y}e^{-\frac{(\ln y - \mu)^2}{2\sigma^2}}, \mbox{ for } y > 0$                                   & $e^{r\mu + \frac{1}{2}r^2 \sigma^2},\ r \geq 0$             & $e^{2\mu + \sigma^2}(e^{\sigma^2}-1)$                                                                              \\ \bottomrule
%    \end{tabular}
%    \vspace{-.7cm}
%\end{table}

\begin{multicols*}{2}
\subsection*{Confidence Intervals}
\subsubsection*{\underline{Estimating Means}}
\underline{For large $r$, $t_{r} \to \mbox{N}(0, 1)$ is a good approximation.}
\subsubsection*{Normal, Single Mean, Known $\sigma$}
$ \left( \bar{x} \pm c \frac{\sigma}{\sqrt{n}} \right) ; \mbox{ with } c=\mbox{F}^{-1}(1-\frac{\alpha}{2}) \mbox{ from pivot } \mbox{N}(0, 1).$
\subsubsection*{Normal, Single Mean, Unknown $\sigma$}
$ \left( \bar{x} \pm c \frac{s}{\sqrt{n}} \right); \mbox{ with } c=\mbox{F}^{-1}(1-\frac{\alpha}{2}) \mbox{ from pivot } t_{n-1}.$
\subsubsection*{Normal, Two Means, Two Known $\sigma$'s}
$ \left( (\bar{x} - \bar{y}) \pm c \sqrt{\frac{\sigma_{X}^{2}}{n} + \frac{\sigma_{Y}^{2}}{m}} \right); \mbox{ with } c \mbox{ from pivot } \mbox{N}(0, 1).$
\subsubsection*{Normal, Two Means, Unknown $\sigma$'s, Many Samples}
$ \left( (\bar{x} - \bar{y}) \pm c \sqrt{\frac{s_{X}^{2}}{n} + \frac{s_{Y}^{2}}{m}} \right); \mbox{ with } c \mbox{ from pivot } \mbox{N}(0, 1).$
\subsubsection*{Normal, Two Means, Unknown $\sigma$'s, Common Variance}
$ \left( (\bar{x} - \bar{y}) \pm c \cdot s_{P} \sqrt{\frac{1}{n} + \frac{1}{m}} \right); \mbox{ with } c \mbox{ from pivot } t_{n+m-2}.$\\
\-\hspace{2cm} $ s_{P} = \sqrt{\frac{(n-1) s^{2}_{X} + (m-1) s^{2}_{Y}}{n+m-2}} $
\subsubsection*{Normal, Two Means, Unknown $\sigma$'s, $\neq$ Variances}
$ \left( (\bar{x} - \bar{y}) \pm c \sqrt{\frac{s_{X}^{2}}{n} + \frac{s_{Y}^{2}}{m}} \right);$ \underline{$\mbox{with } c \mbox{ from pivot } t_{r}.$}\\
\-\hspace{1cm} $ r = \left( \frac{s_{X}^{2}}{n} + \frac{s_{Y}^{2}}{m} \right)^2 / \left( \frac{s_{X}^{4}}{n^{2}(n-1)} + \frac{s_{Y}^{4}}{m^{2}(m-1)} \right) $
\subsubsection*{Normal, Paired Samples}
For pairs $(X_{i}, Y_{i})$, let $D_{i} = X_{i} - Y_{i}$. $D_{i} \sim \mbox{N}(\mu_{D}, \sigma_{D}^{2}).$\\
$ \left( \bar{d} \pm c \frac{s_{d}}{\sqrt{n}} \right);$ \underline{$\mbox{ with } c \mbox{ from pivot } t_{n-1}.$}

\subsubsection*{\underline{Estimating Variance}}
\subsubsection*{Normal, Single Variance - \underline{\color{red} estimate of $\sigma^{2}$ not $\sigma$!}}
$ \left( \frac{(n-1) s^{2}}{b}, \frac{(n-1) s^{2}}{a} \right); \mbox{ with } a, b \mbox{ from pivot } \chi^{2}_{n-1}.$
\subsubsection*{Normal, Two Variances}
A confidence interval for the ratio of the variances $\sigma_{X}^{2} / \sigma_{Y}^{2}$ is
$ \left( a \cdot \frac{s_{x}^{2}}{s_{y}^{2}}, b \cdot \frac{s_{x}^{2}}{s_{y}^{2}} \right); \mbox{ with } a, b \mbox{ from pivot } \mbox{F}_{m-1,n-1}.$

\subsubsection*{\underline{Estimating Proportions (Large n - Normal Approx.)}}
\subsubsection*{Single Proportion}
$ \approx \left( \hat{p} \pm c \sqrt{\frac{\hat{p} (1-\hat{p})}{n}} \right); \mbox{ with } c \mbox{ from pivot } \mbox{N}(0, 1).$
\subsubsection*{Two Proportions}
$ \approx \left( \hat{p_{1}} - \hat{p_{2}} \pm c \sqrt{\frac{\hat{p_{1}} (1-\hat{p_{1}})}{n_{1}} + \frac{\hat{p_{2}} (1-\hat{p_{2}})}{n_{2}}} \right); c \mbox{ from pivot } \mbox{N}(0, 1).$\\
Can also derive a confidence interval from the exact distribution of the binomial RV $n \cdot \hat{p} \sim \mbox{Bi}(n, p)$.

\subsubsection*{\underline{Prediction Intervals}}
Let $X^{*}$ be a future realisation of $X$.\\
If $X \sim \mbox{N}(\mu, \sigma^{2}), \bar{X} \sim \mbox{N}(\mu, \frac{\sigma^{2}}{n}), \mbox{ and } (\bar{X}-X^{*}) \sim \mbox{N}(0, \sigma^{2} + \frac{\sigma^{2}}{n})$.\\
$\left( \bar{x} \pm c \sqrt{s^{2} + \frac{s^{2}}{n}} \right)$ is a prediction interval with $c$ from $t_{n-1}$.\\
If $\sigma$ is known, use pivot $\mbox{N}(0, 1)$. If $\mu$ is known use $\chi^{2}_{n-1}$.

\noindent\rule{\linewidth}{0.25pt}
\subsection*{Regression}
\subsubsection*{Ordinary Least Square (OLS) Estimators}
All parameters are unbiased and except $\hat{\sigma}^{2}$ are normally distributed (Variances as below).\\
Let $K = \sum_{i=1}^{n}(x_{i}-\bar{x})^{2}$ and $D^{2} = \sum_{i=1}^{n}(Y_{i} - \hat{\alpha}_{0} - \hat{\beta}(x_{i} - \bar{x}))^{2}$:
$$\hat{\alpha}_{0} = \bar{Y}; \quad \hat{\beta} = \frac{\sum_{i=1}^{n}(x_{i}-\bar{x})Y_{i}}{\sum_{i=1}^{n}(x_{i}-\bar{x})^{2}}; \quad \hat{\alpha} = \hat{\alpha}_{0} - \hat{\beta}\bar{x}; \quad \hat{\sigma}^{2} = \frac{D^{2}}{n-2}$$
$$\mbox{Var}(\hat{\alpha}) = \left( \frac{1}{n} + \frac{\bar{x}^{2}}{K} \right) \sigma^{2}; \qquad \mbox{Var}(\hat{\beta}) = \frac{\sigma^{2}}{K}; \qquad \mbox{Var}(\hat{\alpha}_{0}) = \frac{\sigma^{2}}{n}$$
$$\mbox{Cov}(\hat{\alpha}_{0}, \hat{\beta}) = 0; \qquad \mbox{Var}(\hat{\mu}(x)) = \left( \frac{1}{n} + \frac{(x-\bar{x})^{2}}{K} \right) \sigma^{2}$$
\subsubsection*{Regression Pivots}
Notice that all the $t_{n-2}$ distributed pivots are estimate $\div$ SE.
$$\frac{(n-2)\hat{\sigma}^{2}}{\sigma^{2}} \sim \chi^{2}_{n-2}; \quad \frac{\hat{\beta} - \beta}{\hat{\sigma} / \sqrt{K}} \sim t_{n-2}; \quad \frac{\hat{\mu}(x) - \mu(x)}{\hat{\sigma} \sqrt{\frac{1}{n} + \frac{(x - \bar{x})^{2}}{K}}} \sim t_{n-2}$$
$$\frac{\hat{\alpha} - \alpha}{\hat{\sigma} \sqrt{\frac{1}{n} + \frac{\bar{x}^{2}}{K}}} \sim t_{n-2}; \qquad \frac{\hat{\alpha}_{0} - \alpha_{0}}{\hat{\sigma} / \sqrt{n}} \sim t_{n-2}$$

\noindent\rule{\linewidth}{0.25pt}
\subsection*{Distribution Free Methods}
\subsubsection*{Sign Test}
\textbf{Hypotheses:} $H_{0}: m = m_{0}; \quad H_{1}: m \neq m_{0}$ or 1 sided $H_{1}$.\\
Let $Y = \sum_{i=1}^{n} I(X_{i} - m_{0} > 0)$. Under $H_{0}$, $Y \sim \mbox{Bi}(n, 0.5)$. Can calculate $p$ values or a critical region from $Y \sim \mbox{Bi}(n, 0.5)$.\\
\textbf{Paired Samples:} Replace $(x_{i}, y_{i})$ with $\mbox{sgn}(x_{i} - y_{i})$ and use the same distribution to check for equal medians. 
\subsubsection*{Wilcoxon Signed Rank / One Sample Test}
\textbf{Hypotheses:} $H_{0}: m = m_{0}; \quad H_{1}: m \neq m_{0}$ or 1 sided $H_{1}$.\\
Rank the $|X_{i} - m_{0}|$ from $1 \to n$ starting at 1 and replace $X_{i}$ with $\mbox{sgn}(X_{i} - m_{0}) \cdot \mbox{rank}(|X_{i} - m_{0}|)$. Let $W$ be the sum of the signed ranks. Under $H_{0}$:
$$Z = \frac{W - 0}{\sqrt{n(n+1)(2n+1) / 6}} \approx \mbox{N}(0, 1)$$
For paired samples we can take the difference and test for equality of medians. When tied ranks occur give them each the average of the ranks they span.
\subsubsection*{Wilcoxon Rank Sum / Two Sample Test}
\textbf{Hypotheses:} $H_{0}: m_{X} = m_{Y}; \quad H_{1}: \bar{H}_{0}$ or 1 sided $H_{1}$.\\
Order the combined sample and let $W$ be the sum of the ranks of $Y_{1}, \dots, Y_{n_{Y}}$. $W$ is approximately normal with:
$$\mathbb{E}(W) = \frac{n_{Y} (n_{X} + n_{Y} + 1)}{2}; \: \mbox{Var}(W) = \frac{n_{X} n_{Y} (n_{X} + n_{Y} + 1)}{12}$$

\noindent\rule{\linewidth}{0.25pt}
\subsection*{Bayesian Inference}
\underline{\color{red} \textsc{Use the LIKELIHOOD not the PDF!}}
\subsubsection*{Law of Total Probability}
$f(x) = \int_{-\infty}^{\infty} f(x, y) dy = \int_{-\infty}^{\infty} f(x \mid y)f(y) dy$
\subsubsection*{Normal Distribution, Known $\sigma$, Inference for $\mu$}
$X_{1}, \dots, X_{n} \sim \mbox{N}(\mu, \sigma^{2})$. Let $Y = \bar{X} \sim \mbox{N}(\mu, \sigma^{2}/n)$.\\
Prior: $\mu \sim \mbox{N}(\mu_{0}, \sigma^{2}_{0})$\\
Posterior: $f(\mu \mid y) \propto f(y \mid \mu) f(\mu) \propto \mbox{exp}\left[ -\frac{(\mu - \mu_{1})^{2}}{2 \sigma^{2}_{1}} \right]$\\
Where:
$$\mu_{1} = \frac{\frac{\mu_{0}}{\sigma^{2}_{0}} + \frac{y}{\sigma^{2}/n}}{\frac{1}{\sigma^{2}_{0}} + \frac{1}{\sigma^{2}/n}}; \qquad \frac{1}{\sigma^{2}_{1}} = \frac{1}{\sigma^{2}_{0}} + \frac{1}{\sigma^{2} / n}$$
So $\mu \mid y \sim \mbox{N}(\mu_{1}, \sigma^{2}_{1})$
\subsubsection*{Binomial Distribution, Beta / Uniform Prior}
$X \sim \mbox{Bi}(n, \theta)$. Prior: $\theta \sim \mbox{Beta}(\alpha, \beta)$\\
Posterior: $\theta \mid x \sim \mbox{Beta}(\alpha + x, \beta + n - x)$
\subsubsection*{Pseudodata}
Gamma prior: $\gamma(\alpha, \beta)$ where $\alpha$ is the total count over all samples and $\beta$ is the number of samples taken.\\
Beta prior: $\mbox{Beta}(\alpha, \beta)$ where $\alpha$ is the number of successes and $\beta$ is the number of failures.

\noindent\rule{\linewidth}{0.25pt}
\subsection*{Pivots}
Sampling from a normal distribution:
$$\frac{\bar{X} - \mu}{\sigma / \sqrt{n}} \sim \mbox{N}(0, 1); \quad \frac{\bar{X} - \mu}{s / \sqrt{n}} \sim t_{n-1}; \quad \frac{(n-1)S^{2}}{\sigma^{2}} \sim \chi^{2}_{n-1}$$

\newpage
\subsection*{ANOVA}
All populations assumed to have equal variance.
\subsubsection*{\underline{F-Statistics / F-test}}
To test any $H_{0}$ in ANOVA, use the F statistic. Since the $MS$ terms are $\chi^{2}$ distributed, $F = MS(X) \div MS(E)$ is distributed as $\mbox{F}_{df_{X}, df_{E}}$ and the rejection region is $F > c$.\\
\textit{eg.} To test $H_{0AB}: \gamma_{ij} = 0\ \forall\ i, j$ use $\mbox{F}_{(a-1)(b-1), ab(c-1)}$.

\subsubsection*{\underline{Single Factor (One Way) ANOVA}}
Total Sample Size: $n = n_{1} + \dots + n_{k}$\\
\textbf{Means}: $$\bar{X}_{i\cdot} = \frac{1}{n_{i}}\sum_{j=1}^{n_{i}} X_{ij}; \qquad \bar{X}_{\cdot \cdot} = \frac{1}{n}\sum_{i=1}^{k} \sum_{j=1}^{n_{i}} X_{ij} = \frac{1}{n}\sum_{i=1}^{k} n_{i}\bar{X}_{i\cdot}$$
\textbf{Hypotheses}: $H_{0}: \mu_{1} = \mu_{2} = \dots = \mu_{k}$ vs. $H_{1}: \bar{H}_{0}$\\
\textbf{Sum of Squares}:\\
Treatment SS:\\
$SS(T) = \sum_{i=1}^{k} \sum_{j=1}^{n_{i}} (\bar{X}_{i\cdot} - \bar{X}_{\cdot \cdot})^{2} = \sum_{i=1}^{k} n_{i} (\bar{X}_{i\cdot} - \bar{X}_{\cdot \cdot})^{2}$\\
Error SS:\\
$SS(E) = \sum_{i=1}^{k} \sum_{j=1}^{n_{i}} (X_{ij} - \bar{X}_{i\cdot})^{2} = \sum_{i=1}^{k} (n_{i} - 1) S_{i}^{2}$\\
Total SS:\\
$SS(TO) = \sum_{i=1}^{k} \sum_{j=1}^{n_{i}} (X_{ij} - \bar{X}_{\cdot \cdot})^{2} = SS(T) + SS(E)$\\
\textbf{Degrees of Freedom}:\\
\centerline{$\mbox{Treatment}: k-1; \qquad \mbox{Error}: n-k$}
\textbf{Null Distributions of Sum of Squares Terms}:
$$\frac{SS(T)}{\sigma^{2}} \sim \chi^{2}_{k-1}; \quad \frac{SS(E)}{\sigma^{2}} \sim \chi^{2}_{n-k}; \quad \frac{SS(TO)}{\sigma^{2}} \sim \chi^{2}_{n-1}$$

\subsubsection*{\underline{Two Factor (Two Way) ANOVA}}
Assume $X_{ij} \sim N(\mu_{ij}, \sigma^{2})$. $\mu_{ij} = \mu + \alpha_{i} + \beta_{j}$. $\sum_{i=1}^{a} \alpha_{i} = 0$ and $\sum_{j=1}^{b} \beta_{j} = 0$. Take one observation from each combination of $a$ and $b$ ($n = ab$).\\
\textbf{Hypotheses}: $H_{0A}: \alpha_{1} = \alpha_{2} = \dots = \alpha_{k} = 0$ vs. $H_{1}: \bar{H}_{0}$\\
or $H_{0B}: \beta_{1} = \beta_{2} = \dots = \beta_{k} = 0$ vs. $H_{1}: \bar{H}_{0}$\\
\textbf{Means}:
$$\bar{X}_{\cdot \cdot} = \frac{1}{ab} \sum_{i=1}^{a} \sum_{j=1}^{b} X_{ij}; \quad \bar{X}_{i \cdot} = \frac{1}{b} \sum_{j=1}^{b} X_{ij}; \quad \bar{X}_{\cdot j} = \frac{1}{a} \sum_{i=1}^{a} X_{ij}$$
\textbf{Sum of Squares}:\\
$SS(A) = b \sum_{i=1}^{a} (\bar{X}_{i\cdot} - \bar{X}_{\cdot \cdot})^{2}$\\
$SS(B) = a \sum_{j=1}^{b} (\bar{X}_{\cdot j} - \bar{X}_{\cdot \cdot})^{2}$\\
Error SS:\\
$SS(E) = \sum_{i=1}^{a} \sum_{j=1}^{b} (X_{ij} - \bar{X}_{i\cdot} - \bar{X}_{\cdot j} + \bar{X}_{\cdot \cdot})^{2}$\\
Total SS:\\
$SS(TO) = SS(A) + SS(B) + SS(E)$\\
\textbf{Degrees of Freedom}:\\
\centerline{$A: a-1; \qquad B: b-1; \qquad \mbox{Error}: (a-1)(b-1)$}

\subsubsection*{\underline{Two Factor ANOVA with Interaction Terms}}
Take samples over two factors, but $c$ samples for each factor pair. $\mu_{ij} = \mu + \alpha_{i} + \beta_{j} + \gamma_{ij}$.\\
\textbf{Hypotheses}: $H_{0A}: \alpha_{1} = \alpha_{2} = \dots = \alpha_{k} = 0$ vs. $H_{1}: \bar{H}_{0}$\\
or $H_{0B}: \beta_{1} = \beta_{2} = \dots = \beta_{k} = 0$ vs. $H_{1}: \bar{H}_{0}$\\
or $H_{0AB}: \gamma_{ij} = 0\ \forall\ i, j$ vs. $H_{1}: \bar{H}_{0}$\\
\textbf{Means}:
$$\bar{X}_{i j \cdot} = \frac{1}{c} \sum_{k=1}^{c} X_{ijk}; \quad \bar{X}_{i \cdot \cdot} = \frac{1}{bc} \sum_{j=1}^{b} \sum_{k=1}^{c} X_{ijk}$$
$$ \bar{X}_{\cdot j \cdot} = \frac{1}{ac} \sum_{i=1}^{a} \sum_{k=1}^{c} X_{ijk}; \quad \bar{X}_{\cdot \cdot \cdot} = \frac{1}{abc} \sum_{i=1}^{a} \sum_{j=1}^{b} \sum_{k=1}^{c} X_{ijk}$$
\textbf{Sum of Squares}:\\
$SS(A) = bc \sum_{i=1}^{a} (\bar{X}_{i \cdot \cdot} - \bar{X}_{\cdot \cdot \cdot})^{2}$\\
$SS(B) = ac \sum_{j=1}^{b} (\bar{X}_{\cdot j \cdot} - \bar{X}_{\cdot \cdot \cdot})^{2}$\\
$SS(AB) = c \sum_{i=1}^{a} \sum_{j=1}^{b} (\bar{X}_{i j \cdot} - \bar{X}_{i \cdot \cdot} - \bar{X}_{\cdot j \cdot} + \bar{X}_{\cdot \cdot \cdot})^{2}$\\
Error SS:\\
$SS(E) = \sum_{i=1}^{a} \sum_{j=1}^{b} \sum_{k=1}^{c} (X_{ijk} - \bar{X}_{i j \cdot})^{2}$\\
Total SS:\\
$SS(TO) = SS(A) + SS(B) + SS(AB) + SS(E)$\\
\textbf{Degrees of Freedom}:\\
\centerline{$A: a-1; \quad B: b-1; \quad AB: (a-1)(b-1); \quad \mbox{Error}: ab(c-1)$}

\subsubsection*{Mean Squares / Mean Square Error}
MSE is found by dividing the $SS(E)$ by its degrees of freedom.\\
\underline{$\hat{\sigma}^{2} = MS(E)$ is an unbiased estimator for the variance.} 

\noindent\rule{\linewidth}{0.25pt}
\subsection*{Distribution of Quantiles and Order Statistics}
\subsubsection*{CDF of $X_{(k)}$}
$$G_{k}(x) = \mbox{Pr}(X_{k} \leq x) = \sum_{i=k}^{n} \binom{n}{i} F(x)^{i} (1 - F(x))^{n-i}$$
\subsubsection*{PDF of $X_{(k)}$}
$$g_{k}(x) = k \binom{n}{k} F(x)^{k-1} (1 - F(x))^{n-k} f(x)$$
\subsubsection*{Asymptotic Distribution of $\hat{\pi}_{p}$}
$$\hat{\pi}_{p} \approx \mbox{N}\left(\pi_{p}, \frac{p(1-p)}{n \cdot f(\pi_{p})^{2}}\right); \qquad \hat{M} \approx \mbox{N}\left(m, \frac{1}{4n \cdot f(m)^{2}}\right)$$

\noindent\rule{\linewidth}{0.25pt}
\subsection*{Goodness-of-fit Test ($\chi^{2}$)}
$O_{i}$ is the Observed count of data in class $i$, $E_{i}$ {\color{red} ($> 5$)} is the Expected count under $H_{0}$. Be careful to use the count and not the proportion. For $k$ classes and $e$ estimated parameters:
$$Q_{k-1-e} = \sum_{i=1}^{k} \frac{(O_{i} - E_{i})^{2}}{E_{i}} \approx \chi^{2}_{k-1-e}$$
Since the numerator $(O_{i} - E_{i})^{2}$ will be larger when $H_{0}$ is false, we reject $H_{0}$ for $Q_{k-1-e} > c$, with $c$ from $\chi^{2}_{k-1-e}$.
\subsubsection*{Two Classes $(k = 2)$}
Testing $H_{0}: p = p_{1}$ vs. $H_{1}: p \neq p_{1}$
\subsubsection*{More than Two Classes $(k > 2)$}
Let $p_{1}, \dots, p_{k}$ define the proportions of a categorical distribution. $H_{0}: ``p_{1}, \dots, p_{k} \mbox{ do define the distribution}"$ vs. $H_{1}: \bar{H}_{0}$

\noindent\rule{\linewidth}{0.25pt}
\subsection*{Sufficient Statistics}
\subsubsection*{Exponential Family}
\centerline{$f(x \mid \theta) = \mbox{exp}\{K(x)p(\theta) + S(x) + q(\theta)\}$}
Has $\sum_{i=1}^{n} K(X_{i})$ as a sufficient statistic for $\theta$.
\subsubsection*{Factorisation Theorem}
$Y = g(x_{1}, \dots, x_{n})$ is sufficient for $\theta$ iff:\\
\centerline{$f(x_{1}, \dots, x_{n} \mid \theta) = \phi\{g(x_{1}, \dots, x_{n}) \mid \theta\} h(x_{1}, \dots, x_{n})$}

\noindent\rule{\linewidth}{0.25pt}
\subsection*{Other Formulae}
\subsubsection*{Sample Variance}
$s^2 = \frac{1}{n-1} \sum_{i=1}^{n} (x_{i}-\bar{x})^2 = \frac{1}{n-1} \left( \left( \sum_{i=1}^{n} x_{i}^2 \right) -n \bar{x}^2 \right)$
\subsubsection*{Cramér-Rao Lower Bound}
The CR Lower Bound is the minimum possible variance of an estimator $\hat{\theta}$ of $\theta$. It is the asymptotic variance of the MLE.
\vspace{-0.2cm}
{\setlength{\mathindent}{0.5cm}
\begin{alignat*}{4}
    &\ell(\theta) = \ln L(\theta); &&\qquad U(\theta) &&= \frac{\partial \ell}{\partial \theta} &&\mbox{\quad (Score Function)}\\
    &V(\theta) = -\frac{\partial U}{\partial \theta}; &&\qquad I(\theta) &&= \mathbb{E}(V(\theta)) &&\mbox{\quad (Fisher Information)}\\
    &\mbox{Var}(\hat{\theta}) \geq \frac{1}{I(\theta)} && && &&\mbox{\quad (CR Lower Bound)}
\end{alignat*} \vspace{-0.5cm}}\\
\noindent In the Fisher Information, take $\mathbb{E}(V(\theta))$ over all $x$, not $\theta$.
\subsubsection*{Gamma Function in Beta + $\gamma$ Distributions}
$\Gamma(n) = (n-1)!$
\end{multicols*}
\end{document}